$p\to q\equiv\neg q\to\neg p$
If we can prove that the negation 

### Example: Prove that for any integer $n$ if $3n+2$ is odd, then $n$ is odd.

This theorem is of the form $p\to q$. What is $p$ and $q$?

$p$: $3n+2$ is odd.
$q$: $n$ is odd.

Contrapositive $\neg q\to\neg p$

$\neg q$: $n$ is even.
$\neg p$: $3n+2$ is even.

Proof:
Assume $n$ is even. Therefore, $n=2k$, where $k$ is an integer.
Now,
$$
\begin{align}
3n+2 \\
\equiv <substitution> \\
3(2k)+2 \\
\equiv <algebra> \\
6k+2 \\
\equiv <algebra> \\
2(3k+1) \\
\equiv <substitution> \\
2j
\end{align}
$$
Since $j$ is an integer, $3n+2$ is even. Therefore, $\neg q\to\neg p$. Therefore $p\to q$.