A direct proof of a conditional statement $p\to q$ is constructed by
- Assume $p$ is true
- Use rules of inferences, axioms, and logical (basic) equivalences to show that $q$ must follow

Ex: Give a direct proof of the theorem "If $n$ is an odd integer, then $n^2$ is odd."

$Def^n$: An integer $n$ is said to be even if there exists an integer $k$ such that $n=2k$

$Def^n$: An integer $n$ is said to be odd if there exists an integer $k$ such that $n=2k+1$

For direct proof, we will assume the hypothesis is true.

Proof:
Assume $n$ is odd, then we have $n=2k+1$, for some integer $k$ (this is essentially a universal instantiation)

Squaring $n$, $n^2$, we get $n^2=2t+1$ where $t$ is an integer


