# Definition
Easier proof than the others (usually), you just basically basic equivalence your way through it.
$$\overline{A\cup(B\cap C)}=(\overline{C}\cup\overline{B})\cap\overline{A}$$
Using set identities

$$\begin{align}
\overline{A\cup(B\cap C)} \\
\equiv<\text{DeMorgan's}> \\
\overline{A}\cap(\overline{B\cap C}) \\
\equiv<\text{DeMorgan's}> \\
\overline{A}\cap(\overline{B}\cup \overline{C}) \\
\equiv<\text{commutative x2}> \\
(\overline{C}\cup\overline{B})\cap\overline{A} \\
\end{align}$$
$$\therefore \overline{A\cup(B\cap C)}=(\overline{C}\cup\overline{B})\cap\overline{A}$$
